moved things around so LS doesn't need to be unfolded
reification speedup by changing some "apply"s in to "simpl apply"s

added an example that needs an unfolding lemma

reify/reverse_defs.v
@@ -1,10 +1,6 @@
 Require Import floyd.proofauto.
-Require Import types.
-Require Import functions.
 Require Export progs.reverse.
 Require Export progs.list_dt.
-Require Import sep.
-Require Import wrapExpr.
 Local Open Scope logic.
 
 (*Some definitions needed from the example file (verif_reverse.v) *)
@@ -253,4 +249,92 @@ Definition Delta :=
                            main_post prog u))) PTree.Leaf) None PTree.Leaf)))).
 
 
-
+Definition Delta2 :=
+(PTree.Node
+           (PTree.Node
+              (PTree.Node
+                 (PTree.Node
+                    (PTree.Node PTree.Leaf (Some (tptr t_struct_list, false))
+                       PTree.Leaf) None PTree.Leaf) None
+                 (PTree.Node
+                    (PTree.Node PTree.Leaf (Some (tptr t_struct_list, true))
+                       PTree.Leaf) None PTree.Leaf)) None
+              (PTree.Node PTree.Leaf None
+                 (PTree.Node PTree.Leaf (Some (tptr t_struct_list, true))
+                    PTree.Leaf))) None
+           (PTree.Node PTree.Leaf None
+              (PTree.Node
+                 (PTree.Node
+                    (PTree.Node PTree.Leaf (Some (tptr t_struct_list, true))
+                       PTree.Leaf) None PTree.Leaf) None PTree.Leaf)),
+        PTree.empty type, tptr t_struct_list,
+        PTree.Node
+          (PTree.Node
+             (PTree.Node
+                (PTree.Node PTree.Leaf
+                   (Some
+                      (Global_func
+                         (WITH _ : unit PRE  [(1%positive, tptr tvoid),
+                          (2%positive, tptr tvoid), 
+                          (3%positive, tuint), (4%positive, tuint)]
+                          (fun _ : environ => !!False) POST  [tvoid]
+                          (fun _ : environ => !!False)))) PTree.Leaf) None
+                PTree.Leaf) None
+             (PTree.Node
+                (PTree.Node
+                   (PTree.Node PTree.Leaf
+                      (Some
+                         (Global_func
+                            (WITH x : share * list int * val PRE 
+                             [(_p, tptr t_struct_list)]
+                             (let (p0, p) := x in
+                              let (sh0, contents0) := p0 in
+                              PROP  ()
+                              LOCAL  (`(eq p) (eval_id _p))
+                              SEP 
+                              (`(lseg LS sh0 (map Vint contents0) p nullval)))
+                             POST  [tint]
+                             (let (p0, _) := x in
+                              let (_, contents0) := p0 in
+                              local (`(eq (Vint (sum_int contents0))) retval)))))
+                      PTree.Leaf) None PTree.Leaf) None PTree.Leaf)) None
+          (PTree.Node
+             (PTree.Node
+                (PTree.Node PTree.Leaf
+                   (Some
+                      (Global_func
+                         (WITH _ : unit PRE  [(1%positive, tptr tschar),
+                          (2%positive, tint)](fun _ : environ => !!False)
+                          POST  [tint](fun _ : environ => !!False))))
+                   PTree.Leaf) None
+                (PTree.Node
+                   (PTree.Node PTree.Leaf
+                      (Some
+                         (Global_func
+                            (WITH x : share * list val * val PRE 
+                             [(_p, tptr t_struct_list)]
+                             (let (p0, p) := x in
+                              let (sh0, contents0) := p0 in
+                              PROP  (writable_share sh0)
+                              LOCAL  (`(eq p) (eval_id _p))
+                              SEP  (`(lseg LS sh0 contents0 p nullval)))
+                             POST  [tptr t_struct_list]
+                             (let (p0, _) := x in
+                              let (sh0, contents0) := p0 in
+                              `(lseg LS sh0 (rev contents0)) retval `nullval))))
+                      PTree.Leaf)
+                   (Some (Global_var (Tarray t_struct_list 3 noattr)))
+                   PTree.Leaf)) None
+             (PTree.Node PTree.Leaf
+                (Some
+                   (Global_func
+                      (WITH _ : unit PRE  [(1%positive, tdouble)]
+                       (fun _ : environ => !!False) POST  [tdouble]
+                       (fun _ : environ => !!False))))
+                (PTree.Node
+                   (PTree.Node PTree.Leaf
+                      (Some
+                         (Global_func
+                            (WITH u : unit PRE  []main_pre prog u POST 
+                             [tint]main_post prog u))) PTree.Leaf) None
+                   PTree.Leaf)))).
