reify/reverse_reify_auto.v
@@ -9,6 +9,54 @@ Require Import preproc.
 
 Local Open Scope logic.
 
+
+Lemma unfold_entail :
+name _p ->
+name _v ->
+name _w ->
+name _t ->
+forall (sh : share) (contents : list val),
+  writable_share sh ->
+  forall (cts1 cts2 : list val) (w v : val),
+    isptr v ->
+   exists (a : Share.t) (b : val),
+     PROP  (contents = rev cts1 ++ cts2)
+     LOCAL  (tc_environ Delta2; `(eq w) (eval_id _w); 
+     `(eq v) (eval_id _v))
+     SEP  (`(lseg LS sh cts1 w nullval); `(lseg LS sh cts2 v nullval))
+     |-- local (tc_expr Delta2 (Etempvar _v (tptr t_struct_list))) &&
+         (`(field_at a t_struct_list _tail b)
+            (eval_expr (Etempvar _v (tptr t_struct_list))) * TT).
+Proof.
+intros.
+eexists; eexists.
+go_lower0.
+Time rcancel.
+Abort. (*we need a lemma!*)
+
+Lemma while_entail2 :
+  name _t ->
+  name _p ->
+  name _s ->
+  name _h ->
+  forall (sh : share) (contents : list int),
+  PROP  ()
+  LOCAL  (tc_environ Delta;
+         `eq (eval_id _t) (eval_expr (Etempvar _p (tptr t_struct_list)));
+         `eq (eval_id _s) (eval_expr (Econst_int (Int.repr 0) tint)))
+  SEP  (`(lseg LS sh (map Vint contents)) (eval_id _p) `nullval)
+          |-- EX  cts : list int,
+  PROP  ()
+  LOCAL 
+        (`(eq (Vint (Int.sub (sum_int contents) (sum_int cts)))) (eval_id _s))
+  SEP  (TT; `(lseg LS sh (map Vint cts)) (eval_id _t) `nullval).
+Proof.
+intros.
+go_lower0.
+Time rcancel.
+rewrite Int.sub_idem. auto. 
+Qed.
+
 Lemma while_entail1 :
   name _t ->
   name _p ->
@@ -32,7 +80,7 @@ Proof.
 intros.
 go_lower0.
 rewrite Int.sub_idem. unfold Int.zero.
-rcancel.
+Time rcancel.
 Qed.
 
 Lemma load_entail1 : 
@@ -55,10 +103,19 @@ Lemma load_entail1 :
           (eval_expr (Etempvar _t (tptr t_struct_list))) * TT).
 Proof.
 intros. 
-eexists. eexists. 
+eexists. eexists.
 go_lower0.
+Time rcancel.
+Qed.
+
+Goal forall contents sh rho,
+(eval_id _t rho) = (eval_id _p rho) ->
+lseg LS sh (map Vint contents) (eval_id _t rho) nullval * emp |--
+lseg LS sh (map Vint contents) (eval_id _p rho) nullval * emp.
+intros.
 rcancel.
 Qed.
+
 
 (* trying to test if my reified hints are usable by Mirror *)
 Goal forall T sh id y, field_at sh T id y nullval |-- !!False && emp.
@@ -115,14 +172,6 @@ intros.
 rcancel.
 Qed.
 
-Goal forall contents sh rho,
-(eval_id _t rho) = (eval_id _p rho) ->
-lseg LS sh (map Vint contents) (eval_id _t rho) nullval * emp |--
-lseg LS sh (map Vint contents) (eval_id _p rho) nullval * emp.
-intros.
-rcancel.
-Qed.
-
 Goal forall a ,
  !!True && a
    |-- !!True &&
@@ -143,24 +192,4 @@ intros.
 rcancel.
 Qed.
 
-Lemma while_entail2 :
-  name _t ->
-  name _p ->
-  name _s ->
-  name _h ->
-  forall (sh : share) (contents : list int),
-  PROP  ()
-  LOCAL  (tc_environ Delta;
-         `eq (eval_id _t) (eval_expr (Etempvar _p (tptr t_struct_list)));
-         `eq (eval_id _s) (eval_expr (Econst_int (Int.repr 0) tint)))
-  SEP  (`(lseg LS sh (map Vint contents)) (eval_id _p) `nullval)
-          |-- EX  cts : list int,
-  PROP  ()
-  LOCAL 
-        (`(eq (Vint (Int.sub (sum_int contents) (sum_int cts)))) (eval_id _s))
-  SEP  (TT; `(lseg LS sh (map Vint cts)) (eval_id _t) `nullval).
-Proof.
-intros.
-go_lower0.
-(*Not there yet...*)
-Abort.
+
